Progress on PermuteProgproofs.v

x86/PermuteProgproof.v
@@ -7,8 +7,10 @@
 Require Import Coqlib Errors.
 Require Import Integers Floats AST.
 Require Import Values Memory Events Globalenvs Smallstep.
+Require Import LocalLib.
 Require Import Permutation.
 Require Import Asm RealAsm.
+Require Import AsmInject.
 
 (** matching modulo the permutation of definitions *)
 
@@ -27,7 +29,11 @@ Qed.
 (** Preservation of semantics under permutation *)
 Section PRESERVATION.
 
+Existing Instance inject_perm_all.
 Context `{external_calls_prf: ExternalCalls}.
+
+Local Existing Instance mem_accessors_default.
+
 
 Variable prog: Asm.program.
 Variable tprog: Asm.program.
@@ -36,9 +42,288 @@ Hypothesis TRANSF: match_prog prog tprog.
 Let ge := Genv.globalenv prog.
 Let tge := Genv.globalenv tprog.
 
-Theorem transf_program_correct:
-  forward_simulation (RealAsm.semantics prog (Pregmap.init Vundef))
-                     (RealAsm.semantics tprog (Pregmap.init Vundef)).
+
+Record match_inj (j: meminj) : Type :=
+  {
+    (** Preservation of finding of global symbols *)
+    agree_find_symbol:
+      forall id b,
+        Genv.find_symbol ge id = Some b ->
+        exists b', Genv.find_symbol tge id = Some b' /\
+              j b = Some (b', 0);
+
+    (** Preservation of finding of external functions *)
+    agree_find_funct_ptr:
+      forall b f ofs b',
+        Genv.find_funct_ptr ge b = Some f ->
+        j b = Some (b', ofs) ->
+        Genv.find_funct_ptr tge b' = Some f;
+  }.
+
+Inductive match_states : Asm.state -> Asm.state -> Prop :=
+|match_states_intro: forall j m m' rs rs'
+   (MINJ: Mem.inject j (def_frame_inj m) m m')
+   (RSINJ: regset_inject j rs rs')
+   (MATCH_INJ: match_inj j) ,
+   match_states (Asm.State rs m) (Asm.State rs' m').
+
+(* Definition shift_inj n (j: positive -> option positive) : positive -> option positive := *)
+(*   fun b => if plt n b then None *)
+(*         else  *)
+(*           match j (Pos.sub b n) with *)
+(*           | None => None *)
+(*           | Some m => Some (Pos.add n m) *)
+(*           end. *)
+
+(* Eval compute in (Pos.sub 1%positive 3%positive). *)
+
+(* Fixpoint perm_inj_match {A} (l1 l2: list A) (pm: Permutation l1 l2) (j: positive -> option positive) : Prop := *)
+(*   match pm with *)
+(*   | perm_nil => forall b, j b = Some b *)
+(*   | perm_skip x l1' l2' pm' =>  *)
+(*     exists j', perm_inj_match l1' l2' pm' j' /\ *)
+(*           fun b => if zeq b 0 then 0 else  *)
+(*             shift_inj 1 j' b *)
+(*   | perm_swap x y l => *)
+(*     fun b => if zeq b 0 then 1 *)
+(*           else if zeq b 1 then 0 *)
+(*                else b *)
+(*   | perm_trans l l' l'' pm1 pm2 => *)
+(*     let j1 := perm_inj_fun l l' pm1 in *)
+(*     let j2 := perm_inj_fun l' l'' pm2 in *)
+(*     fun b => j2 (j1 b) *)
+(*   end. *)
+    
+
+Lemma find_symbol_pres_some: forall id b, 
+    Genv.find_symbol ge id = Some b ->
+    exists b', Genv.find_symbol tge id = Some b'.
 Admitted.
+
+Lemma find_symbol_pres_none: forall id, 
+    Genv.find_symbol ge id = None ->
+    Genv.find_symbol tge id = None.
+Admitted.
+
+
+Theorem step_simulation:
+  forall S1 t S2, step ge S1 t S2 ->
+                  forall S1' (MS: match_states S1 S1'),
+                    (exists S2', step tge S1' t S2' /\ match_states S2 S2').
+Proof.
+(*   destruct 1; intros; inv MS. *)
+  
+(*   - (* Internal Step *) *)
+(*     exploit exec_instr_simulation; eauto. *)
+(*     intros (m2' & rs2' & EXEC & EXT & RS & STK). *)
+(*     exists (State rs2' m2'). split; [|constructor; auto]. *)
+(*     eapply exec_step_internal; eauto. *)
+(*     red in H8. generalize (H8 PC). rewrite H. *)
+(*     inversion 1. eauto. *)
+(*     rewrite find_funct_ptr_transf. auto. *)
+  
+(*   - (* Builtin step *) *)
+(*     exploit eval_builtin_args_lessdef''; eauto. *)
+(*     intros (vargs' & EB & VLE). *)
+(*     exploit external_call_mem_extends; eauto. *)
+(*     intros (vres' & m2' & EC & VLER & EXT & UCHG). *)
+(*     eexists. split. *)
+(*     eapply exec_step_builtin; eauto. *)
+(*     red in H10. generalize (H10 PC). *)
+(*     rewrite H. inversion 1. eauto. *)
+(*     rewrite find_funct_ptr_transf. auto. *)
+(*     eapply eval_builtin_args_preserved with (ge1 := ge); eauto. *)
+(*     intros. rewrite find_symbol_transf. auto. *)
+(*     eapply external_call_symbols_preserved; eauto. exact senv_equiv. *)
+(*     constructor; eauto. *)
+(*     erewrite <- (external_call_stack_blocks _ _ _ m'0 _ _ m2'); eauto. *)
+(*     erewrite <- (external_call_stack_blocks _ _ _ m _ _ m'); eauto. *)
+
+(*   - (* External Step *) *)
+(*     edestruct extcall_arguments_match as (args' & EXTARGS & VLE). *)
+(*     Focus 3. exact H1. *)
+(*     instantiate (1:= rs'0 # RSP <- (Val.offset_ptr (rs'0 RSP) (Ptrofs.repr (size_chunk Mptr)))). *)
+(*     eapply regset_lessdef_pregset; eauto. *)
+(*     eauto. *)
+(*     exploit external_call_mem_extends; eauto. *)
+(*     intros (vres' & m2' & EXTCALL & VLER & EXT2 & CHG). *)
+(*     eexists. split. *)
+(*     eapply exec_step_external; eauto. *)
+(*     red in H9. generalize (H9 PC). rewrite H. *)
+(*     inversion 1. eauto. *)
+(*     rewrite find_funct_ptr_transf. auto. *)
+(*     red in H9. generalize (H9 RSP). inversion 1; congruence. *)
+(*     edestruct Mem.loadv_extends as (ra' & LV & VLRA).  *)
+(*     exact H7. exact LOADRA. red in H9. eauto. *)
+(*     inv VLRA; congruence. *)
+(*     red in H9. generalize (H9 RSP). *)
+(*     intros VLRSP. inv VLRSP; congruence. *)
+(*     apply external_call_symbols_preserved with ge; eauto. *)
+(*     exact senv_equiv. *)
+(*     constructor; auto. *)
+(*     erewrite <- (external_call_stack_blocks _ _ _ m'0 _ _ m2'); eauto. *)
+(*     erewrite <- (external_call_stack_blocks _ _ _ m _ _ m'); eauto. *)
+(*     (** Regset lessdef *) *)
+(*     eapply regset_lessdef_pregset; eauto. *)
+(*     eapply regset_lessdef_pregset; eauto. *)
+(* Qed. *)
+Admitted.
+
+
+Lemma init_mem_transf: forall m,
+    Genv.init_mem prog = Some m ->
+    exists m' j, Genv.init_mem tprog = Some m' /\ Mem.inject j (def_frame_inj m) m m'.
+Proof.
+(*   unfold Genv.init_mem. *)
+(*   intros m ALLOC. *)
+(*   red in TRANSF. unfold transf_program in TRANSF. *)
+(*   replace (prog_defs tprog) with (map transf_globdef (prog_defs prog)). *)
+(*   Focus 2. rewrite TRANSF. cbn. auto. *)
+(*   apply alloc_globals_extends with ge Mem.empty; eauto. *)
+(*   intros. rewrite find_symbol_transf. auto. *)
+(*   eapply Mem.extends_refl. *)
+(* Qed. *)
+Admitted.
+
+(* Lemma initial_state_inject: forall m m' rs st prog prog', *)
+(*     (forall b, Genv.find_symbol (Genv.globalenv prog) b = Genv.find_symbol (Genv.globalenv prog') b) -> *)
+(*     prog_main prog = prog_main prog' -> *)
+(*     Mem.stack m = nil -> *)
+(*     Mem.stack m' = nil -> *)
+(*     Mem.inject j m m' -> *)
+(*     initial_state_gen prog rs m st -> *)
+(*     exists st', initial_state_gen prog' rs m' st' /\ match_states st st'. *)
+(* Proof. *)
+(*   intros m m' rs st prog0 prog' FS MAIN ISNIL ISNIL' EXT IS. *)
+(*   inv IS. *)
+(*   assert (exists m1' : mem, Mem.alloc (Mem.push_new_stage m') 0  *)
+(*                                  (Mem.stack_limit + align (size_chunk Mptr) 8) = (m1', bstack) *)
+(*                        /\ Mem.extends m1 m1') as MALLOC'. *)
+(*   { eapply Mem.alloc_extends; eauto. *)
+(*     eapply Mem.extends_push; eauto.  *)
+(*     omega. omega. *)
+(*   } *)
+(*   destruct MALLOC' as (m1' & MALLOC' & EXT1). *)
+(*   generalize (Mem.alloc_stack_blocks _ _ _ _ _ MALLOC). *)
+(*   intros ISNIL1.  *)
+(*   rewrite Mem.push_new_stage_stack in ISNIL1. *)
+(*   rewrite ISNIL in ISNIL1. *)
+(*   generalize (Mem.alloc_stack_blocks _ _ _ _ _ MALLOC'). *)
+(*   intros ISNIL1'.  *)
+(*   rewrite Mem.push_new_stage_stack in ISNIL1'. *)
+(*   rewrite ISNIL' in ISNIL1'. *)
+(*   assert (inject_perm_condition Freeable) as IPF. *)
+(*   { red. cbn. auto. } *)
+(*   generalize (Mem.drop_extends _ _ _ _ _ _ _ EXT1 IPF MDROP). *)
+(*   intros (m2' & MDROP' & EXT2). *)
+(*   generalize (Mem.drop_perm_stack _ _ _ _ _ _ MDROP). *)
+(*   intros ISNIL2. rewrite ISNIL1 in ISNIL2. *)
+(*   generalize (Mem.drop_perm_stack _ _ _ _ _ _ MDROP'). *)
+(*   intros ISNIL2'. rewrite ISNIL1' in ISNIL2'. *)
+(*   assert (exists m3', Mem.record_stack_blocks  *)
+(*                    m2' (make_singleton_frame_adt' bstack RawAsm.frame_info_mono 0) = Some m3' /\ Mem.extends m3 m3')  *)
+(*     as MRSB'. *)
+(*   {  *)
+(*     eapply Mem.record_stack_blocks_extends; eauto. *)
+(*     * rewrite ISNIL2'. auto. *)
+(*     * red. unfold make_singleton_frame_adt'. simpl. *)
+(*       intros b fi o k p BEQ PERM. inv BEQ; try contradiction. *)
+(*       inv H0. unfold RawAsm.frame_info_mono. simpl. *)
+(*       erewrite drop_perm_perm in PERM; eauto. destruct PERM. *)
+(*       eapply Mem.perm_alloc_3; eauto. *)
+(*     * red. repeat rewrite_stack_blocks. constructor. auto. *)
+(*     * repeat rewrite_stack_blocks. *)
+(*       rewrite ISNIL, ISNIL'. omega. *)
+(*   }  *)
+(*   destruct MRSB' as (m3' & MRSB' & EXT3). *)
+(*   generalize (Mem.record_stack_blocks_stack _ _ _ _ _ MRSB ISNIL2). *)
+(*   intros ISNIL3. *)
+(*   generalize (Mem.record_stack_blocks_stack _ _ _ _ _ MRSB' ISNIL2'). *)
+(*   intros ISNIL3'. *)
+
+(*   assert (exists m4', Mem.storev Mptr m3'  *)
+(*                            (Vptr bstack (Ptrofs.repr (Mem.stack_limit + align (size_chunk Mptr) 8 - size_chunk Mptr))) Vnullptr = Some m4'  *)
+(*                 /\ Mem.extends m4 m4') as STORE_RETADDR'. *)
+(*   { eapply Mem.storev_extends; eauto. } *)
+(*   destruct STORE_RETADDR' as (m4' & STORE_RETADDR' & EXT4). *)
+(*   generalize (Mem.storev_stack _ _ _ _ _ STORE_RETADDR). *)
+(*   intros ISNIL4. rewrite ISNIL3 in ISNIL4. *)
+(*   generalize (Mem.storev_stack _ _ _ _ _ STORE_RETADDR'). *)
+(*   intros ISNIL4'. rewrite ISNIL3' in ISNIL4'. *)
+(*   exists (State rs0 m4'). split. *)
+(*   - econstructor; eauto. *)
+(*     rewrite <- FS. rewrite <- MAIN. auto. *)
+(*   - eapply match_states_intro; eauto. congruence. *)
+(*     apply regset_lessdef_refl. *)
+(* Qed. *)
+
+Lemma transf_initial_states:
+  forall st1 rs, initial_state prog rs st1 ->
+         exists st2, initial_state tprog rs st2 /\ match_states st1 st2.
+Proof.
+(*   intros st1 rs HInit. *)
+(*   inv HInit. *)
+(*   generalize (init_mem_transf _ H). *)
+(*   intros (m' & j & INIT & MINJ). *)
+(*   assert (exists st', initial_state_gen tprog rs m' st' /\ match_states st1 st') as IS. *)
+(*   { apply initial_state_extends with m prog; eauto. *)
+(*     intros. rewrite find_symbol_transf. auto. *)
+(*     rewrite prog_main_eq. auto. *)
+(*     erewrite Genv.init_mem_stack; eauto. *)
+(*     erewrite Genv.init_mem_stack; eauto. *)
+(*   } *)
+(*   destruct IS as (st1' & IS & MS). *)
+(*   exists st1'. split; eauto. *)
+(*   econstructor; eauto. *)
+(* Qed. *)
+Admitted.
+
+
+Lemma transf_final_states:
+  forall st1 st2 r,
+  match_states st1 st2 -> final_state st1 r -> final_state st2 r.
+Proof.
+  intros st1 st2 r MS HFinal.
+  inv HFinal.
+  inv MS.
+  econstructor; eauto.
+  red in RSINJ. generalize (RSINJ PC).
+  rewrite H. inversion 1. auto.
+  red in RSINJ. generalize (RSINJ RAX).
+  rewrite H0. inversion 1. subst. auto.
+Qed.
+
+
+
+Theorem transf_program_correct: forall rs,
+  forward_simulation (RealAsm.semantics prog rs)
+                     (RealAsm.semantics tprog rs).
+Proof.
+  intro rs.
+  apply forward_simulation_step with match_states.
+  - intros id. unfold match_prog in TRANSF.
+    decompose [and] TRANSF.
+    cbn.
+    unfold Genv.public_symbol.
+    symmetry.
+    destr.
+    + exploit find_symbol_pres_some; eauto.
+      intros (b' & FSYM).
+      unfold tge in FSYM.
+      rewrite FSYM. 
+      unfold Genv.globalenv.
+      repeat rewrite Genv.genv_public_add_globals. 
+      rewrite <- H2. auto.
+    + exploit find_symbol_pres_none; eauto.
+      intros FSYM. 
+      unfold tge in FSYM. rewrite FSYM. auto.
+  - simpl. intros s1 Hinit.
+    exploit transf_initial_states; eauto.
+  - simpl. intros s1 s2 r MS HFinal. eapply transf_final_states; eauto.
+  - simpl. intros s1 t s1' STEP s2 MS.
+    edestruct step_simulation as (STEP' & MS' ); eauto.
+Qed.
+  
+
 
 End PRESERVATION.
